\documentclass{article} % latex file 
\usepackage[margin={1in}]{geometry}
\usepackage{logicproof}
\usepackage{amsmath}
\usepackage{amssymb}
\usepackage{graphicx}
\graphicspath{ {./images/} }

\title{CSU44004 Formal Verification: Natural Deduction Solutions}
\author{By: Alexander Sepelenco}
\date{} % no date

\begin{document}

\maketitle

\section*{Note}

This document will contain 9 years of propositional natural deduction solutions ranging from 2022 to 2015.

\section*{2022 Q2}

\paragraph{(a)}

Prove: $\vdash (A \to B) \lor (B \to A)$
\begin{logicproof}{3}
    \begin{subproof}
        \neg ((A \to B) \lor (B \to A)) & assumption\\
        \begin{subproof}
            A \to B & assumption\\
            (A \to B) \lor (B \to A) & $\lor\mathrm{i}_1$, 2\\
            \bot & $\neg\mathrm{e}$, 3, 1
        \end{subproof}
        \neg (A \to B) & $\neg\mathrm{i}$, 2--4\\
        \begin{subproof}
            B & assumption\\
            \begin{subproof}
                A & assumption\\
                B & copy 6
            \end{subproof}
            A \to B & $\to\mathrm{i}$, 7--8\\
            \bot & $\neg\mathrm{e}$, 9, 5
        \end{subproof}
        \neg B & $\neg\mathrm{i}$, 6--10\\
        \begin{subproof}
            \neg A & assumption\\
            \neg B & copy 11
        \end{subproof}
        \neg A \to \neg B & $\to\mathrm{i}$, 12--13\\
        \begin{subproof}        
            B & assumption\\
            \neg\neg A & $MT$, 15, 14\\
            A & $\neg\neg\mathrm{e}$, 16
        \end{subproof}        
        B \to A & $\to\mathrm{i}$, 15--17\\
        (A \to B) \lor (B \to A) & $\lor\mathrm{i}_2$, 18\\
        \bot & $\neg\mathrm{e}$, 19, 1 
    \end{subproof}
    \neg \neg ((A \to B) \lor (B \to A)) & $\neg\mathrm{i}$, 1--20\\
    (A \to B) \lor (B \to A) & $\neg\neg\mathrm{e}$, 21 
\end{logicproof}

\newpage

\section*{2021 Q2}

I will create a helper proof for this problem to make it easier for myself.
Use this proof as a reference as I will not repeat this proof in the solutions.\\
I will call this rule $\neg\to\mathrm{e}$\\
Prove: $\neg (p \to q) \vdash p \land \neg q$
\begin{logicproof}{3}
    \neg (p \to q) & premise\\
    \begin{subproof}
        \neg (p \land \neg q) & assumption\\
        \begin{subproof}
            p & assumption\\
            \begin{subproof}
                \neg q & assumption\\
                p \land \neg q & $\land\mathrm{i}$, 3, 4\\
                \bot & $\neg\mathrm{e}$, 5, 2
            \end{subproof}
            \neg\neg q & $\neg\mathrm{i}$, 4--6\\
            q & $\neg\neg\mathrm{e}$, 6
        \end{subproof}
        p \to q & $\to\mathrm{i}$, 3--7\\
        \bot & $\neg\mathrm{e}$, 9, 1
    \end{subproof}
    \neg\neg (p \land \neg q) & $\neg\mathrm{i}$, 2--10\\ 
    p \land \neg q & $\neg\neg\mathrm{e}$, 12
\end{logicproof}

\paragraph{(a)}

Prove: $\neg q, t \to q, \neg r \to \neg s, p \to u, \neg t \to \neg r, u \to s \vdash p \to x$
\begin{logicproof}{1}
    \neg q & premise\\
    t \to q & premise\\
    \neg r \to \neg s & premise\\
    p \to u & premise\\
    \neg t \to \neg r & premise\\
    u \to s & premise\\
    \begin{subproof}
        \neg (p \to x) & assumption\\
        p \land \neg x & $\neg\to\mathrm{e}$, 7\\
        \neg t & $MT$, 1, 2\\
        \neg r & $\to\mathrm{e}$, 9, 5\\
        \neg s & $\to\mathrm{e}$, 10, 3\\
        \neg u & $MT$, 11, 6\\
        \neg p & $MT$, 12, 4\\
        p & $\land\mathrm{e}_1$, 8\\
        \bot & $\neg\mathrm{e}$, 14, 13
    \end{subproof}
    \neg\neg (p \to x) & $\neg\mathrm{i}$, 7--15\\
    p \to x & $\neg\neg\mathrm{e}$, 16 
\end{logicproof}

\newpage

\section*{2020 Q2}
\paragraph{(a)}

This solution is ever so slightly different to 2021 Q2 (a), so I will do it slightly differently
for practice.\\
Prove: $t \to q, \neg r \to \neg s, p \to u, \neg t \to \neg r, u \to s \vdash p \to q$
\begin{logicproof}{1}
    t \to q & premise\\
    \neg r \to \neg s & premise\\
    p \to u & premise\\
    \neg t \to \neg r & premise\\
    u \to s & premise\\
    \begin{subproof}
        \neg (p \to q) & assumption\\
        p \land \neg q & $\neg\to\mathrm{e}$, 6\\
        \neg q & $\land\mathrm{e}_2$, 7\\
        p & $\land\mathrm{e}_1$, 7\\
        \neg t & $MT$, 8, 1\\
        \neg r & $\to\mathrm{e}$, 10, 4\\
        \neg s & $\to\mathrm{e}$, 11, 2\\
        \neg u & $MT$, 12, 5\\
        \neg p & $MT$, 13, 3\\
        \bot & $\neg\mathrm{e}$, 14, 9 
    \end{subproof}
    \neg\neg (p \to q) & $\neg\mathrm{i}$, 6--16\\
    p \to q & $\neg\neg\mathrm{e}$, 16 
\end{logicproof}

\section*{2019 Q3}
\paragraph{(a) (i)}

Prove: $\neg p \to r \vdash \neg r \to p$\\
\begin{logicproof}{1}
    \neg p \to r & premise\\
    \begin{subproof}
        \neg (\neg r \to p) & assumption\\
        \neg r \land \neg p & $\neg\to\mathrm{e}$, 2\\
        \neg p & $\land\mathrm{e}_2$, 3\\
        r & $\to\mathrm{e}$, 4, 1\\
        \neg r & $\land\mathrm{e}_1$, 3
    \end{subproof}
    \bot & $\neg\mathrm{e}$, 5, 6
\end{logicproof}

\paragraph{(a) (ii)}

Prove: $\neg (p \to r) \to \neg q \vdash q \to p \to r$
\begin{logicproof}{1}
    \neg (p \to r) \to \neg q & premise\\
    \begin{subproof}
        \neg (q \to p \to r) & assumption\\
        q \land \neg (p \to r) & $\neg\to\mathrm{e}$, 2\\
        \neg (p \to r) & $\land\mathrm{e}_2$, 3\\
        \neg q & $\to\mathrm{e}$, 4, 1\\
        q & $\land\mathrm{e}_1$, 3\\
        \bot & $\neg\mathrm{e}$, 6, 5
    \end{subproof}
    \neg \neg (q \to p \to r) & $\neg\mathrm{i}$, 2--7\\
    q \to p \to r & $\neg\neg\mathrm{e}$, 8
\end{logicproof}

\section*{2019 Q1}
\paragraph{(c) (i)}

Prove: $p \land q \to \neg r \vdash r \to p \to \neg q$
\begin{logicproof}{1}
    p \land q \to \neg r & premise\\
    \begin{subproof}
        \neg (r \to p \to \neg q) & assumption\\
        r \land \neg (p \to \neg q) & $\neg\to\mathrm{e}$, 2\\
        r & $\land\mathrm{e}_1$, 3\\
        \neg (p \to \neg q) & $\land\mathrm{e}_2$, 3\\
        p \land \neg\neg q & $\neg\to\mathrm{e}$, 5\\
        p & $\land\mathrm{e}_1$, 6\\
        \neg\neg q & $\land\mathrm{e}_2$, 6\\
        q & $\neg\neg\mathrm{e}$, 8\\
        p \land q & $\land\mathrm{i}$, 7, 8\\
        \neg r & $\to\mathrm{e}$, 10, 1\\
        \bot & $\neg\mathrm{e}$, 4, 11
    \end{subproof}
    \neg\neg (r \to p \to \neg q) & $\neg\mathrm{i}$, 2--12\\
    r \to p \to \neg q & $\neg\neg\mathrm{e}$, 13 
\end{logicproof}
\paragraph{(c) (ii)}
Sorry, this question is our assignment. I cannot give the answer to this one.

\section*{2018 Q1}
\paragraph{(c) (i)}

Prove: $\vdash \neg ((p \to \neg p) \land (\neg p \to p))$
\begin{logicproof}{3}
    \begin{subproof}
        \neg (\neg ((p \to \neg p) \land (\neg p \to p))) & assumption\\
        \begin{subproof}
            (p \to \neg p) \land (\neg p \to p) & assumption\\
            p \to \neg p & $\land\mathrm{e}_1$, 2\\
            \neg p \to p & $\land\mathrm{e}_2$, 2\\
            \begin{subproof}
                p & assumption\\
                \neg p & $\to\mathrm{e}$, 5, 3\\
                \bot & $\neg\mathrm{e}$, 5, 6
            \end{subproof}
            \neg p & $\neg\mathrm{i}$, 5--7\\
            p & $\to\mathrm{e}$, 8, 4\\
            \bot & $\neg\mathrm{e}$, 9, 8
        \end{subproof}
        \neg ((p \to \neg p) \land (\neg p \to p)) & $\neg\mathrm{i}$, 2--11\\
        \bot & $\neg\mathrm{e}$, 11, 1
    \end{subproof}
    \neg\neg (\neg ((p \to \neg p) \land (\neg p \to p))) & $\neg\mathrm{i}$, 1--12\\
    \neg ((p \to \neg p) \land (\neg p \to p)) & $\neg\neg\mathrm{e}$, 13
\end{logicproof}

\newpage

\paragraph{(c) (ii)}

Prove: $p \to (q \lor r) \vdash (p \to q) \lor (p \to r)$
\begin{logicproof}{2}
    p \to (q \lor r) & assumption\\
    \begin{subproof}
        \neg ((p \to q) \lor (p \to r)) & assumption\\
        \begin{subproof}
            p \to q & assumption\\
            (p \to q) \lor (p \to r) & assumption\\
            \bot & $\neg\mathrm{e}$, 4, 5
        \end{subproof}
        \neg (p \to q) & $\neg\mathrm{i}$, 3--5\\
        p \land \neg q & $\neg\to\mathrm{e}$, 6\\
        p & $\land\mathrm{e}_1$, 7\\
        (q \lor r) & $\to\mathrm{e}$, 8, 1\\
        \neg q & $\land\mathrm{e}_2$, 7\\
        \begin{subproof}
            p \to r & assumption\\
            (p \to q) \lor (p \to r) & $\lor\mathrm{i}_2$, 11\\
            \bot & $\neg\mathrm{e}$, 12, 2
        \end{subproof}
        \neg (p \to r) & $\neg\mathrm{i}$, 11-13\\
        p \land \neg r & $\neg\to\mathrm{e}$, 14\\
        \neg r & $\land\mathrm{e}_2$, 15\\
        \begin{subproof}
            q & assumption\\
            \neg q & copy 10\\
            \bot & $\neg\mathrm{e}$, 17, 18
        \end{subproof}
        \begin{subproof}
            r & assumption\\
            \neg r & copy 16\\
            \bot & $\neg\mathrm{e}$, 16 
        \end{subproof}
        \bot & $\lor\mathrm{e}$, 9, 17--9, 20-22
    \end{subproof}
    \neg\neg ((p \to q) \lor (p \to r)) & $\neg\mathrm{i}$, 2--23\\
    (p \to q) \lor (p \to r) & $\neg\neg\mathrm{e}$, 24
\end{logicproof}

\section*{2017 Q1}

\paragraph{(c) (i)}

Prove: $p \to r \vdash \neg p \lor r$
\begin{logicproof}{2}
    p \to r & premise\\
    \begin{subproof}
    \neg (\neg p \lor r) & assumption\\
        \begin{subproof}
            p & assumption\\
            r & $\to\mathrm{e}$, 3, 1\\
            \neg p \lor r & $\lor\mathrm{i}_2$, 4\\
            \bot & $\neg\mathrm{e}$, 5, 2
        \end{subproof}
        \neg p & $\neg\mathrm{i}$, 3--6\\
        \neg p \lor r & $\lor\mathrm{i}_1$, 7\\
        \bot & $\neg\mathrm{e}$, 8, 2
    \end{subproof}
    \neg\neg (\neg p \lor r) & $\neg\mathrm{i}$, 2--9\\
    \neg p \lor r & $\neg\neg\mathrm{e}$, 10
\end{logicproof}

\newpage

\paragraph{(c) (ii)}

Prove: $(\neg p \to r), (r \to p), (p \to s) \vdash p \land s$
\begin{logicproof}{2}
    \neg p \to r & premise\\
    r \to p & premise\\
    p \to s & premise\\
    \begin{subproof}
        \neg (p \land s) & assumption\\
        \begin{subproof}
            p & assumption\\
            s & $\to\mathrm{e}$, 5, 3\\
            p \land s & $\land\mathrm{i}$, 5, 6\\
            \bot & $\neg\mathrm{e}$, 7, 4
        \end{subproof}
        \neg p & $\neg\mathrm{i}$, 5--8\\
        r & $\to\mathrm{e}$, 9, 1\\
        p & $\to\mathrm{e}$, 10, 2\\
        \bot & $\neg\mathrm{e}$, 11, 9
    \end{subproof}
    \neg\neg (p \land s) & $\neg\mathrm{i}$, 4--12\\
    p \land s & $\neg\neg\mathrm{e}$, 13
\end{logicproof}

\section*{2016 Q1}
I will prove Morgan's Theorem using natural deduction to use as a helper rule for the problem (ii).\\
I will call this rule $DM_2$\\
Prove: $\neg (p \lor q) \vdash \neg p \land \neg q$
\begin{logicproof}{2}
    \neg (p \lor q) & premise\\
    \begin{subproof}
        \neg (\neg p \land \neg q) & assumption\\
        \begin{subproof}
            p & assumption\\
            p \lor q & $\lor\mathrm{i}_1$, 3\\
            \bot & $\neg\mathrm{e}$, 4, 1
        \end{subproof}
        \neg p & $\neg\mathrm{i}$, 3--5\\
        \begin{subproof}
            q & assumption\\
            p \lor q & $\lor\mathrm{i}_2$, 7\\
            \bot & $\neg\mathrm{e}$, 8, 1
        \end{subproof}
        \neg q & $\neg\mathrm{i}$, 7--9\\
        \neg p \land \neg q & $\land\mathrm{i}$, 6, 10\\
        \bot & $\neg\mathrm{e}$, 11, 2
    \end{subproof}
    \neg\neg (\neg p \land \neg q) & $\neg\mathrm{i}$, 2--12\\
    \neg p \land \neg q & $\neg\neg\mathrm{e}$, 13
\end{logicproof}

\newpage

\paragraph{(d) (i)}

Prove: $p \lor (q \land r) \vdash (p \lor q) \land (p \lor r)$
\begin{logicproof}{3}
    p \lor (q \land r) & premise\\
    \begin{subproof}
        \neg ((p \lor q) \land (p \lor r)) & assumption\\
        \begin{subproof}
            p \lor q & assumption\\
            \begin{subproof}
                p \lor r & assumption\\
                (p \lor q) \land (p \lor r) & $\land\mathrm{i}$, 3, 4\\
                \bot & $\neg\mathrm{e}$, 5, 2
            \end{subproof}
            \neg (p \lor r) & $\neg\mathrm{i}$, 4--6\\
            \neg p \land \neg r & $DM_2$, 7\\
            \neg p & $\land\mathrm{e}_1$, 8\\
            \neg r & $\land\mathrm{e}_2$, 8\\
            \begin{subproof}
                p & assumption\\
                \neg p & copy 9\\
                \bot & $\neg\mathrm{e}$, 11, 12
            \end{subproof}
            \begin{subproof}
                (q \lor r) & assumption\\
                r & $\land\mathrm{e}_2$, 14\\
                \bot & $\neg\mathrm{e}$, 15, 10
            \end{subproof}
            \bot & $\lor\mathrm{e}$, 1, 11--13, 14--16
        \end{subproof}
        \neg (p \lor q) & $\neg\mathrm{i}$, 2--17\\
        \neg p \land \neg q & $DM_2$, 18\\
        \neg p & $\land\mathrm{e}_1$, 19\\
        \neg q & $\land\mathrm{e}_2$, 19\\
        \begin{subproof}
            p & assumption\\
            \bot & $\neg\mathrm{e}$, 22, 20 
        \end{subproof}
        \begin{subproof}
            (q \land r) & assumption\\
            q & $\land\mathrm{e}_1$, 24\\
            \bot & $\neg\mathrm{e}$, 24, 21 
        \end{subproof}
        \bot & $\lor\mathrm{e}$, 1, 22--23, 24--26
    \end{subproof}
    \neg\neg ((p \lor q) \land (p \lor r)) & $\neg\mathrm{i}$, 2--27\\
    (p \lor q) \land (p \lor r) & $\neg\neg\mathrm{e}$, 28
\end{logicproof}

\paragraph{(d) (ii)}

Prove: $\phi \land \neg \psi \to \neg \phi \vdash \phi \to \psi$
\begin{logicproof}{1}
    \phi \land \neg \psi \to \neg \phi & premise\\
    \begin{subproof}
        \neg (\phi \to \psi) & assumption\\
        \phi \land \neg \psi & $\neg\to\mathrm{e}$, 2\\ 
        \neg \phi & $\to\mathrm{e}$, 3, 1\\
        \phi & $\land\mathrm{e}_1$, 3\\
        \bot & $\neg\mathrm{e}$, 4, 5
    \end{subproof}
    \neg\neg (\phi \to \psi) & $\neg\mathrm{i}$, 2--6\\
    \phi \to \psi & $\neg\neg\mathrm{e}$, 7
\end{logicproof}

\section*{2015 Q1}

\paragraph{(e) (i)}

Prove: $(\phi_1 \to \psi_1), (\neg \psi_2 \to \neg \phi_2) \vdash (\phi_1 \land \phi_2) \to (\phi_1 \lor \phi_2)$
\begin{logicproof}{2}
    (\phi_1 \to \psi_1) & premise\\
    (\neg \psi_2 \to \neg \phi_2) & premise\\
    \begin{subproof}
        \neg ((\phi_1 \land \phi_2) \to (\psi_1 \lor \psi_2)) & assumption\\
        \begin{subproof}
            \phi_1 \land \phi_2 & assumption\\
            \phi_1 & $\land\mathrm{e}_1$, 4\\
            \psi_1 & $\to\mathrm{e}$, 5, 1\\
            \psi_1 \lor \psi_2 & $\lor\mathrm{i}$, 6
        \end{subproof}
        (\phi_1 \land \phi_2) \to \psi_1 \lor \psi_2 & $\to\mathrm{i}$, 4--7\\
        \bot & $\neg\mathrm{e}$, 8, 3
    \end{subproof}
    \neg\neg ((\phi_1 \land \phi_2) \to (\psi_1 \lor \psi_2)) & $\neg\mathrm{i}$, 3--9\\
    (\phi_1 \land \phi_2) \to (\psi_1 \lor \psi_2) & $\neg\neg\mathrm{e}$, 10
\end{logicproof}

\paragraph{(e) (ii)}

Prove: $\phi \to \neg \psi \vdash \psi \to \neg \phi$
\begin{logicproof}{1}
    \phi \to \neg \phi & premise\\
    \begin{subproof}
        \neg (\psi \to \neg \phi) & assumption\\
        \psi \land \neg \neg \phi & $\neg\to\mathrm{e}$, 2\\
        \neg\neg \phi & $\land\mathrm{e}_2$, 3\\
        \phi & $\neg\neg\mathrm{e}$, 4\\
        \neg \phi & $\to\mathrm{e}$, 5, 1\\
        \bot & $\neg\mathrm{e}$, 5, 6
    \end{subproof}
    \neg\neg (\psi \to \neg \psi) & $\neg\mathrm{i}$, 2--7\\
    \psi \to \neg \psi & $\neg\neg\mathrm{e}$, 8
\end{logicproof}

\end{document} 
